rocq/theories/TypeSystem/EnvRuntimeShadowSummaryFacts.v
@@ -47,20 +47,28 @@ Definition env_fns_root_shadow_direct_call_provenance_summary_check_ready
     lookup_fn fname (env_fns env) = Some fdef ->
     callee_body_root_shadow_direct_call_provenance_summary env fdef.
 
+Inductive supported_non_type_generic_function_value_call_callee_shape : Ty -> Prop :=
+  | SFV_TFn : forall T param_tys ret,
+      ty_core T = TFn param_tys ret ->
+      supported_non_type_generic_function_value_call_callee_shape T
+  | SFV_TForall_TFn : forall T m bounds body param_tys ret,
+      ty_core T = TForall m bounds body ->
+      ty_core body = TFn param_tys ret ->
+      supported_non_type_generic_function_value_call_callee_shape T.
+
 Definition supported_non_type_generic_function_value_call_callee_ty
     (T : Ty) : Prop :=
-  exists param_tys ret,
-    ty_core T = TFn param_tys ret.
+  supported_non_type_generic_function_value_call_callee_shape T.
 
 Definition supported_non_type_generic_function_value_call_expr
     (env : global_env) (Ω : outlives_ctx) (n : nat)
     (R : root_env) (Γ : ctx) (callee : expr) (args : list expr) : Prop :=
-  exists x T_callee Γ_callee R_callee roots_callee param_tys ret,
+  exists x T_callee Γ_callee R_callee roots_callee,
     callee = EVar x /\
     ECallExpr callee args = ECallExpr (EVar x) args /\
     infer_core_env_roots_shadow_safe env Ω n R Γ (EVar x) =
       infer_ok (T_callee, Γ_callee, R_callee, roots_callee) /\
-    ty_core T_callee = TFn param_tys ret.
+    supported_non_type_generic_function_value_call_callee_shape T_callee.
 
 Definition callee_body_root_shadow_non_capturing_call_provenance_summary
     (env : global_env) (fdef : fn_def) : Prop :=
@@ -85,7 +93,7 @@ Definition callee_body_root_shadow_non_capturing_call_provenance_summary
     ty_compatible_b (fn_outlives fdef) T_body (fn_ret fdef) = true /\
     roots_exclude_params (fn_params fdef) roots_body /\
     root_env_excludes_params (fn_params fdef) R_body) \/
-  exists x args T_callee Γ_callee R_callee roots_callee param_tys ret
+  exists x args T_callee Γ_callee R_callee roots_callee
       T_body Γ_out R_body roots_body,
     fn_body fdef = ECallExpr (EVar x) args /\
     preservation_ready_args args /\
@@ -97,7 +105,7 @@ Definition callee_body_root_shadow_non_capturing_call_provenance_summary
       (fn_body_ctx fdef)
       (EVar x) = infer_ok
         (T_callee, Γ_callee, R_callee, roots_callee) /\
-    ty_core T_callee = TFn param_tys ret /\
+    supported_non_type_generic_function_value_call_callee_shape T_callee /\
     NoDup (ctx_names (params_ctx (fn_params fdef))) /\
     typed_env_roots_shadow_safe
       (global_env_with_local_bounds env (fn_bounds fdef))
